We will prove the proposition

\begin{proposition}
    For any $a,b>1$, there exists an integer $n$ such that
    \[
    a^n > n^b \text{.}
    \]
\end{proposition}

\begin{proof}
    The Taylor series for $a^n$ is given by
    \[
    a^n = \sum_{k=0}^{\infty} \frac{n^k \log^k(a)}{k!}
    \]

    Then
    \begin{align*}
        \lim_{n \to \infty} (a^n - n^b) &= \lim_{n \to \infty} n^b \left( \frac{a^n}{n^b} - 1 \right )\\
            &= \lim_{n \to \infty} n^b \left( \frac{1}{n^b} \sum_{k=0}^{\infty} \frac{n^k\log^k(a)}{k!} - 1 \right)\\
            &= \lim_{n \to \infty} n^b \left(\sum_{k=0}^{\infty} \frac{n^{k-b}\log^k(a)}{k!} -1 \right)\\
            &= \lim_{n \to \infty} n^b \left( \sum_{k=0}^{b-1} \frac{n^{k-b}\log^k(a)}{k!} + \sum_{k=b}^{\infty} \frac{n^{k-b}\log^k(a)}{k!} -1 \right)\\
            &= \lim_{n \to \infty} n^b \left( \sum_{k=0}^{b-1} \frac{n^{k-b}\log^k(a)}{k!} + \sum_{k=b}^{\infty} \frac{n^{k-b}\log^k(a)}{k!} -1 \right)\\
            &= \lim_{n \to \infty} \sum_{k=0}^{b-1} \frac{n^k \log^k(a)}{k!} + \lim_{n \to \infty} n^b \left( \sum_{k=b}^{\infty} \frac{n^{k-b}\log^k(a)}{k!} - 1 \right)\\
            &= \lim_{n \to \infty} \sum_{k=0}^{b-1} \frac{n^k \log^k(a)}{k!} + \lim_{n \to \infty} n^b \cdot \left(\lim_{n \to \infty} \sum_{k=b}^{\infty} \frac{n^{k-b}\log^k(a)}{k!} - \lim_{n \to \infty} 1   \right) \\
            &= \infty + \infty \cdot (\infty - 1)\\
            &= \infty
    \end{align*}

    Since the limit is infinite, there exists some $N$ such that for all $n > N$, $a^n > n^b$.

\end{proof}